

quelles que soient les propositions **A B**,
 $((\neg \mathbf{A} \Rightarrow \mathbf{B}) \Rightarrow (\neg \mathbf{B} \Rightarrow \mathbf{A}))$

Montrons $(\neg \mathbf{A} \Rightarrow \mathbf{B}) \Rightarrow (\neg \mathbf{B} \Rightarrow \mathbf{A})$ (1)

($\Rightarrow I$)

Supposons que $\neg \mathbf{A} \Rightarrow \mathbf{B}$ (h1)

Montrons $\neg \mathbf{B} \Rightarrow \mathbf{A}$ (2)

($\Rightarrow I$)

Supposons que $\neg \mathbf{B}$ (h2)

Montrons \mathbf{A} (3)

(A)

Supposons que $\neg \mathbf{A}$ (h3)

Montrons \perp (4)

($\neg E$)

Montrons \mathbf{B} (5)

($\Rightarrow E$)

Montrons $\neg \mathbf{A}$ (6)

d'après (h3)

Montrons $\neg \mathbf{A} \Rightarrow \mathbf{B}$ (7)

d'après (h1)

Montrons $\neg \mathbf{B}$ (8)

d'après (h2)